Stop using Sinf_term for evaluation of constants

SInfinity/Basic.lean
@@ -2,16 +2,16 @@ import Mathlib.Init.ZeroOne
 import Std.Data.AssocList
 
 inductive Sinf_term where
-  | S_var : String → Sinf_term
+  | var : String → Sinf_term
   | O : Sinf_term
   | S : Sinf_term → Sinf_term
-  | S_plus : Sinf_term → Sinf_term → Sinf_term
-  | S_times : Sinf_term → Sinf_term → Sinf_term
+  | plus : Sinf_term → Sinf_term → Sinf_term
+  | times : Sinf_term → Sinf_term → Sinf_term
 
-prefix:max "_" => Sinf_term.S_var
-prefix:max "S " => Sinf_term.S
-infixl:65 " +ₛ " => Sinf_term.S_plus
-infixl:70 " *ₛ " => Sinf_term.S_times
+prefix:max "_" => Sinf_term.var
+postfix:75 "↗" => Sinf_term.S
+infixl:65 " +ₛ " => Sinf_term.plus
+infixl:70 " *ₛ " => Sinf_term.times
 
 namespace Sinf_term
 
@@ -21,23 +21,23 @@ namespace Sinf_term
 
 @[simp] def eval : Sinf_term → Std.AssocList String Nat → Option Nat :=
   λ t al ↦ match t with
-    | S_var x => Std.AssocList.find? x al
+    | var x => Std.AssocList.find? x al
     | O => some 0
     | S θ => Nat.succ <$> eval θ al
-    | S_plus θ₁ θ₂ => Nat.add <$> eval θ₁ al <*> eval θ₂ al
-    | S_times θ₁ θ₂ => Nat.mul <$> eval θ₁ al <*> eval θ₂ al
+    | plus θ₁ θ₂ => Nat.add <$> eval θ₁ al <*> eval θ₂ al
+    | times θ₁ θ₂ => Nat.mul <$> eval θ₁ al <*> eval θ₂ al
 
 #reduce eval (S O +ₛ _"x" *ₛ _"x") (Std.AssocList.cons "x" 21 Std.AssocList.nil)
 
 @[simp] def subst : Sinf_term → String → Sinf_term → Sinf_term :=
   λ θ' x θ ↦ match θ' with
-  | S_var x' => match String.decEq x x' with
+  | var x' => match String.decEq x x' with
     | isTrue _ => θ
-    | isFalse _ => S_var x'
+    | isFalse _ => var x'
   | O => O
   | S θ' => S (subst θ' x θ)
-  | S_plus θ₁ θ₂ => S_plus (subst θ₁ x θ) (subst θ₂ x θ)
-  | S_times θ₁ θ₂ => S_times (subst θ₁ x θ) (subst θ₂ x θ)
+  | plus θ₁ θ₂ => plus (subst θ₁ x θ) (subst θ₂ x θ)
+  | times θ₁ θ₂ => times (subst θ₁ x θ) (subst θ₂ x θ)
 
 end Sinf_term
 
@@ -49,6 +49,88 @@ instance : Zero Sinf_term where
 
 instance : One Sinf_term where
   one := Sinf_term.S Sinf_term.O
+
+instance : Add Sinf_term where
+  add := Sinf_term.plus
+
+instance : Mul Sinf_term where
+  mul := Sinf_term.times
+
+inductive NoVars : Sinf_term → Type where
+  | O : NoVars Sinf_term.O
+  | S : ∀ {t}, NoVars t → NoVars (t↗)
+  | plus : ∀ {θ₁ θ₂}, NoVars θ₁ → NoVars θ₂ → NoVars (θ₁ +ₛ θ₂)
+  | times : ∀ {θ₁ θ₂}, NoVars θ₁ → NoVars θ₂ → NoVars (θ₁ *ₛ θ₂)
+
+namespace NoVars
+
+theorem fromNat {n : Nat} : NoVars (Sinf_term.fromNat n) := by
+  induction n <;> try constructor <;> assumption
+
+theorem unique {θ : Sinf_term} (nv₁ nv₂ : NoVars θ) : nv₁ = nv₂ := by
+  induction θ <;> try contradiction
+  case O => cases nv₁; cases nv₂; rfl
+  case S θ ih =>
+    cases nv₁; case S nv₁ => cases nv₂; case S nv₂ =>
+    apply congrArg; exact (ih nv₁ nv₂)
+  case plus θ₁ θ₂ ih₁ ih₂ =>
+    cases nv₁; case plus nv₁₁ nv₂₁ => cases nv₂; case plus nv₁₂ nv₂₂ =>
+    apply congrArg₂; exact (ih₁ nv₁₁ nv₁₂); exact (ih₂ nv₂₁ nv₂₂)
+  case times θ₁ θ₂ ih₁ ih₂ =>
+    cases nv₁; case times nv₁₁ nv₂₁ => cases nv₂; case times nv₁₂ nv₂₂ =>
+    apply congrArg₂; exact (ih₁ nv₁₁ nv₁₂); exact (ih₂ nv₂₁ nv₂₂)
+
+end NoVars
+
+inductive Sinf_const where
+  | O : Sinf_const
+  | S : Sinf_const → Sinf_const
+  | plus : Sinf_const → Sinf_const → Sinf_const
+  | times : Sinf_const → Sinf_const → Sinf_const
+
+postfix:75 "↗ᶜ" => Sinf_const.S
+infixl:65 " +ᶜ " => Sinf_const.plus
+infixl:70 " *ᶜ " => Sinf_const.times
+
+namespace Sinf_const
+
+@[simp] def fromNat (n : Nat) : Sinf_const := match n with
+  | Nat.zero => O
+  | Nat.succ n => S (fromNat n)
+
+@[simp] def eval : Sinf_const → Nat :=
+  λ t ↦ match t with
+    | O => 0
+    | S θ => Nat.succ $ eval θ
+    | plus θ₁ θ₂ => Nat.add (eval θ₁) (eval θ₂)
+    | times θ₁ θ₂ => Nat.mul (eval θ₁) (eval θ₂)
+
+@[simp] def coerce (θ : Sinf_term) (nv : NoVars θ) : Sinf_const :=
+  match nv with
+  | NoVars.O => Sinf_const.O
+  | @NoVars.S θ' nv => Sinf_const.S (coerce θ' nv)
+  | @NoVars.plus θ₁' θ₂' nv₁ nv₂ => Sinf_const.plus (coerce θ₁' nv₁) (coerce θ₂' nv₂)
+  | @NoVars.times θ₁' θ₂' nv₁ nv₂ => Sinf_const.times (coerce θ₁' nv₁) (coerce θ₂' nv₂)
+
+#reduce eval (S (S O) +ᶜ S (S (S O) *ᶜ S (S (S O))))
+#reduce coerce (Sinf_term.plus (Sinf_term.S Sinf_term.O) Sinf_term.O) (NoVars.plus (NoVars.S NoVars.O) NoVars.O)
+
+end Sinf_const
+
+instance : Coe Nat Sinf_const where
+  coe := Sinf_const.fromNat
+
+instance : Zero Sinf_const where
+  zero := Sinf_const.O
+
+instance : One Sinf_const where
+  one := Sinf_const.S Sinf_const.O
+
+instance : Add Sinf_const where
+  add := Sinf_const.plus
+
+instance : Mul Sinf_const where
+  mul := Sinf_const.times
 
 inductive Sinf : Type where
   | S_eq : Sinf_term → Sinf_term → Sinf
@@ -78,4 +160,4 @@ notation:45 α " [" x " ≔ " θ "]" => Sinf.subst α x θ
 
 open Sinf_term
 
-#reduce Sinf.subst (¬ₛ S S S S _"x" =ₛ S S O) "x" (O +ₛ S O)
+#reduce Sinf.subst (¬ₛ _"x"↗↗↗↗ =ₛ O↗↗) "x" (O +ₛ O↗)
